Partly_Filled_Array.thy
@@ -1,0 +1,166 @@
+theory Partly_Filled_Array
+  imports
+ "Imperative_Loops"
+ "Refine_Imperative_HOL.IICF_Array_List"
+
+begin
+
+text "An array that is only partly filled.
+The number of actual elements contained is kept in a second element.
+This represents a weakened version of the array_list from IICF"
+
+type_synonym 'a pfarray = "'a array_list"
+
+definition is_pfarray where
+"is_pfarray l \<equiv> \<lambda>(a,n). \<exists>\<^sub>A l'. a \<mapsto>\<^sub>a l' *  \<up>(n \<le> length l' \<and> l = (take n l'))"
+
+  lemma is_pfarray_prec[safe_constraint_rules]: "precise is_pfarray"
+    unfolding is_pfarray_def[abs_def]
+    apply(rule preciseI)
+    apply(simp split: prod.splits) 
+  	using preciseD snga_prec by fastforce
+  
+
+definition "pfa_empty init_cap \<equiv> do {
+  a \<leftarrow> Array.new init_cap default;
+  return (a,0)
+}"
+
+definition "pfa_append \<equiv> \<lambda>(a,n) x. do {
+  a \<leftarrow> Array.upd n x a;
+  return (a,n+1)
+}"
+
+definition "pfa_last \<equiv> arl_last"
+
+definition pfa_butlast :: "'a::heap pfarray \<Rightarrow> 'a pfarray Heap" where
+  "pfa_butlast \<equiv> \<lambda>(a,n).
+    return (a,n-1)
+  "
+
+definition "pfa_get \<equiv> arl_get"
+
+definition "pfa_length \<equiv> arl_length"
+
+definition "pfa_is_empty \<equiv> arl_is_empty"
+
+definition "pfa_set \<equiv> arl_set"
+
+lemma pfa_empty_rule[sep_heap_rules]: "< emp > pfa_empty N <is_pfarray []>"
+  by (sep_auto simp: pfa_empty_def arl_empty_def is_pfarray_def)
+
+lemma pfa_length_rule[sep_heap_rules]: "
+  <is_pfarray l a> 
+    pfa_length a
+  <\<lambda>r. is_pfarray l a * \<up>(r=length l)>"
+  by (sep_auto simp: pfa_length_def arl_length_def is_pfarray_def)
+
+  lemma arl_is_empty_rule[sep_heap_rules]: "
+    <is_pfarray l a> 
+      pfa_is_empty a
+    <\<lambda>r. is_pfarray l a * \<up>(r\<longleftrightarrow>(l=[]))>"
+    by (sep_auto simp: pfa_is_empty_def arl_is_empty_def is_pfarray_def)
+
+lemma pfa_append_rule[sep_heap_rules]: "
+   n < length l \<Longrightarrow>
+    < is_pfarray l (a,n) > 
+      pfa_append (a,n) x 
+    <\<lambda>a. is_pfarray (l@[x]) a >\<^sub>t"  
+    by (sep_auto 
+      simp: pfa_append_def arl_append_def is_pfarray_def take_update_last neq_Nil_conv
+      split: prod.splits nat.split)
+
+lemma pfa_last_rule[sep_heap_rules]: "
+  l\<noteq>[] \<Longrightarrow>
+  <is_pfarray l a> 
+    pfa_last a
+  <\<lambda>r. is_pfarray l a * \<up>(r=last l)>"
+  by (sep_auto simp: pfa_last_def arl_last_def is_pfarray_def last_take_nth_conv)
+
+lemma pfa_butlast_rule[sep_heap_rules]: "
+  <is_pfarray l a> 
+    pfa_butlast a
+  <is_pfarray (butlast l)>\<^sub>t"
+    by (sep_auto 
+      split: prod.splits
+      simp: pfa_butlast_def is_pfarray_def butlast_take)  
+
+
+lemma pfa_get_rule[sep_heap_rules]: "
+  i < length l \<Longrightarrow>
+  < is_pfarray l a> 
+    pfa_get a i
+  <\<lambda>r. is_pfarray l a * \<up>((l!i) = r)>"
+  apply (sep_auto simp: is_pfarray_def pfa_get_def arl_get_def  split: prod.split)
+  done
+
+  lemma pfa_set_rule[sep_heap_rules]: "
+    i<length l \<Longrightarrow>
+    <is_pfarray l a> 
+      pfa_set a i x
+    <is_pfarray (l[i:=x])>"
+    by (sep_auto simp: pfa_set_def arl_set_def is_pfarray_def split: prod.split)
+
+ definition "pfa_assn A \<equiv> hr_comp is_pfarray (\<langle>the_pure A\<rangle>list_rel)"
+  lemmas [safe_constraint_rules] = CN_FALSEI[of is_pure "pfa_assn A" for A]
+
+
+  lemma pfa_assn_comp: "is_pure A \<Longrightarrow> hr_comp (pfa_assn A) (\<langle>B\<rangle>list_rel) = pfa_assn (hr_comp A B)"
+    unfolding pfa_assn_def
+    by (auto simp: hr_comp_the_pure hr_comp_assoc list_rel_compp)
+
+  lemma pfa_assn_comp': "hr_comp (pfa_assn id_assn) (\<langle>B\<rangle>list_rel) = pfa_assn (pure B)"
+    by (simp add: pfa_assn_comp)
+
+context 
+  notes [fcomp_norm_unfold] = pfa_assn_def[symmetric] pfa_assn_comp'
+  notes [intro!] = hfrefI hn_refineI[THEN hn_refine_preI]
+  notes [simp] = pure_def hn_ctxt_def invalid_assn_def
+begin  
+
+
+  lemma pfa_empty_hnr_aux: "(uncurry0 (pfa_empty N),uncurry0 (RETURN op_list_empty)) \<in> unit_assn\<^sup>k \<rightarrow>\<^sub>a is_pfarray"  
+    by sep_auto
+  sepref_decl_impl (no_register) pfa_empty: pfa_empty_hnr_aux .
+
+  definition "op_pfa_empty (N::nat) \<equiv> op_list_empty"
+
+  lemma pfa_length_hnr_aux: "(pfa_length,RETURN o op_list_length) \<in> is_pfarray\<^sup>k \<rightarrow>\<^sub>a nat_assn"
+    by sep_auto
+  sepref_decl_impl pfa_length: pfa_length_hnr_aux .
+
+  lemma pfa_is_empty_hnr_aux: "(pfa_is_empty,RETURN o op_list_is_empty) \<in> is_pfarray\<^sup>k \<rightarrow>\<^sub>a bool_assn"
+    by sep_auto
+  sepref_decl_impl pfa_is_empty: pfa_is_empty_hnr_aux .  
+
+lemma pfa_last_hnr_aux: "(pfa_last,RETURN o op_list_last) \<in> [pre_list_last]\<^sub>a is_pfarray\<^sup>k \<rightarrow> id_assn"
+    by sep_auto
+  sepref_decl_impl pfa_last: pfa_last_hnr_aux . 
+
+  lemma pfa_butlast_hnr_aux: "(pfa_butlast,RETURN o op_list_butlast) \<in> [pre_list_butlast]\<^sub>a is_pfarray\<^sup>d \<rightarrow> is_pfarray"
+    by sep_auto
+  sepref_decl_impl pfa_butlast: pfa_butlast_hnr_aux .
+
+  lemma pfa_get_hnr_aux: "(uncurry pfa_get,uncurry (RETURN oo op_list_get)) \<in> [\<lambda>(l,i). i<length l]\<^sub>a (is_pfarray\<^sup>k *\<^sub>a nat_assn\<^sup>k) \<rightarrow> id_assn"
+    by sep_auto
+  sepref_decl_impl pfa_get: pfa_get_hnr_aux .
+
+  lemma pfa_set_hnr_aux: "(uncurry2 pfa_set,uncurry2 (RETURN ooo op_list_set)) \<in> [\<lambda>((l,i),_). i<length l]\<^sub>a (is_pfarray\<^sup>d *\<^sub>a nat_assn\<^sup>k *\<^sub>a id_assn\<^sup>k) \<rightarrow> is_pfarray"
+    by sep_auto
+  sepref_decl_impl pfa_set: pfa_set_hnr_aux .
+
+  sepref_definition pfa_swap is "uncurry2 mop_list_swap" :: "((pfa_assn id_assn)\<^sup>d *\<^sub>a nat_assn\<^sup>k *\<^sub>a nat_assn\<^sup>k \<rightarrow>\<^sub>a pfa_assn id_assn)"
+    unfolding gen_mop_list_swap[abs_def]
+    by sepref
+  sepref_decl_impl (ismop) pfa_swap: pfa_swap.refine .  
+end
+
+
+lemma [def_pat_rules]: "op_pfa_empty$N \<equiv> UNPROTECT (op_pfa_empty N)" by simp
+interpretation pfa_sz: list_custom_empty "pfa_assn A" "pfa_empty N" "PR_CONST (op_pfa_empty N)"
+  apply unfold_locales
+  apply (rule pfa_empty_hnr)
+  by (auto simp: op_pfa_empty_def)
+
+
+end
